move prophecy trace and stepcount to global_state_interp; add global_state support to FFI; remove prophecy support from goose_lang

src/goose_lang/adequacy.v
@@ -14,20 +14,23 @@ Class ffi_interp_adequacy `{FFI: !ffi_interp ffi} `{EXT: !ext_semantics ext ffi}
     ffiΣ: gFunctors;
     (* modeled after subG_gen_heapPreG and gen_heap_init *)
     subG_ffiPreG : forall Σ, subG ffiΣ Σ -> ffi_preG Σ;
-    ffi_initP: ffi_state → Prop;
+    ffi_initP: ffi_state → ffi_global_state → Prop;
     ffi_update_pre: ∀ Σ, ffi_preG Σ -> ffi_names -> ffiG Σ;
     ffi_update_pre_update: ∀ Σ (hPre: ffi_preG Σ) names1 names2,
         ffi_update Σ (ffi_update_pre _ hPre names1) names2 =
         ffi_update_pre _ hPre names2;
     ffi_update_pre_get: ∀ Σ (hPre: ffi_preG Σ) names,
         ffi_get_names _ (ffi_update_pre _ hPre names) = names;
-    ffi_name_init : forall Σ (hPre: ffi_preG Σ) (σ:ffi_state), ffi_initP σ →
-          ⊢ |==> ∃ (names: ffi_names), let H0 := ffi_update_pre _ hPre names in ffi_ctx H0 σ ∗ ffi_start H0 σ;
+    ffi_name_init : forall Σ (hPre: ffi_preG Σ) (σ:ffi_state) (g:ffi_global_state), ffi_initP σ g →
+          ⊢ |==> ∃ (names: ffi_names), let H0 := ffi_update_pre _ hPre names in
+                   ffi_ctx H0 σ ∗ ffi_global_ctx H0 g ∗ ffi_start H0 σ g;
     ffi_crash : forall Σ,
-          ∀ (σ σ': ffi_state) (CRASH: ext_crash σ σ') (Hold: ffiG Σ),
-           ⊢ ffi_ctx Hold σ ==∗ ∃ (new: ffi_names), ffi_ctx (ffi_update Σ Hold new) σ' ∗
-                                                  ffi_crash_rel Σ Hold σ (ffi_update Σ Hold new) σ' ∗
-                                                  ffi_restart (ffi_update Σ Hold new) σ';
+          ∀ (σ σ': ffi_state) (g: ffi_global_state) (CRASH: ext_crash σ σ') (Hold: ffiG Σ),
+           ⊢ ffi_ctx Hold σ -∗ ffi_global_ctx Hold g ==∗
+             ∃ (new: ffi_names), ffi_ctx (ffi_update Σ Hold new) σ' ∗
+                                 ffi_global_ctx (ffi_update Σ Hold new) g ∗
+                                 ffi_crash_rel Σ Hold σ (ffi_update Σ Hold new) σ' ∗
+                                 ffi_restart (ffi_update Σ Hold new) σ';
   }.
 
 (* this is the magic that lets subG_ffiPreG solve for an ffi_preG using only
@@ -41,7 +44,6 @@ Class heapPreG `{ext: ext_op} `{EXT_SEM: !ext_semantics ext ffi}
   heap_preG_iris :> invPreG Σ;
   heap_preG_crash :> crashPreG Σ;
   heap_preG_heap :> na_heapPreG loc val Σ;
-  heap_preG_proph :> proph_mapPreG proph_id (val * val) Σ;
   heap_preG_ffi : ffi_preG Σ;
   heap_preG_trace :> trace_preG Σ;
 }.
@@ -51,9 +53,6 @@ Definition heap_update_pre Σ `(hpreG : heapPreG Σ) (Hinv: invG Σ) (Hcrash: cr
      heapG_crashG := Hcrash;
      heapG_ffiG := ffi_update_pre Σ (heap_preG_ffi) (heap_ffi_names names);
      heapG_na_heapG := na_heapG_update_pre (heap_preG_heap) (heap_heap_names names);
-     heapG_proph_mapG :=
-       {| proph_map_inG := heap_preG_proph;
-          proph_map_name := (heap_proph_name names) |};
      heapG_traceG := traceG_update_pre Σ (heap_preG_trace) (heap_trace_names names)
  |}.
 
@@ -91,8 +90,10 @@ Ltac solve_inG_deep :=
                            | H:subG _ _ |- _ => move : H; apply subG_inG in H || clear H
                            end; intros; try done; split; assumption || by apply _.
 
-Definition heapΣ `{ext: ext_op} `{ffi_interp_adequacy} : gFunctors := #[invΣ; crashΣ; na_heapΣ loc val; ffiΣ; proph_mapΣ proph_id (val * val); traceΣ].
-Instance subG_heapPreG `{ext: ext_op} `{@ffi_interp_adequacy ffi Hinterp ext EXT} {Σ} : subG heapΣ Σ → heapPreG Σ.
+Definition heapΣ `{ext: ext_op} `{ffi_interp_adequacy} : gFunctors :=
+  #[invΣ; crashΣ; na_heapΣ loc val; ffiΣ; traceΣ].
+Instance subG_heapPreG `{ext: ext_op} `{@ffi_interp_adequacy ffi Hinterp ext EXT} {Σ} :
+  subG heapΣ Σ → heapPreG Σ.
 Proof.
   solve_inG_deep.
 Qed.
